theories/sf_rdes/utp_sfrd_contracts.thy
@@ -9,7 +9,7 @@ definition mk_CRD :: "'s upred \<Rightarrow> ('e list \<Rightarrow> 'e set \<Rig
 
 syntax
   "_ref_var" :: "logic"
-  "_mk_CRD"  :: "uexp \<Rightarrow> uexp \<Rightarrow> logic \<Rightarrow> logic" ("[_/ \<turnstile> _/ | _]\<^sub>C")
+  "_mk_CRD"  :: "logic \<Rightarrow> logic \<Rightarrow> logic \<Rightarrow> logic" ("[_/ \<turnstile> _/ | _]\<^sub>C")
 
 parse_translation \<open>
 let
